src/examples/matmul-opt/GPU.MatMulOpt.Pure.fsti
@@ -10,10 +10,10 @@ let singleton #a (elem: a) : seq a = Seq.cons elem Seq.empty
 
 let rec matmul_single
   (rows shared columns: nat)
-  (s1: (seq U64.t){ Seq.length s1 == rows * shared })
-  (s2 : (seq U64.t){ Seq.length s2 == shared * columns })
+  (s1: (seq u64){ Seq.length s1 == rows * shared })
+  (s2 : (seq u64){ Seq.length s2 == shared * columns })
   (row: nat{row < rows}) (col: nat{col < columns}) (to: nat)
-    : GTot U64.t (decreases to)
+    : GTot u64 (decreases to)
   =
   if reveal to > shared then 0UL else if reveal to = 0 then 0UL else
     (
@@ -24,8 +24,8 @@ let rec matmul_single
 #push-options "--retry 2" 
 let matmul_single_lemma
   (rows shared columns: nat)
-  (s1: (seq U64.t){ Seq.length s1 == rows * shared })
-  (s2 : (seq U64.t){ Seq.length s2 == shared * columns })
+  (s1: (seq u64){ Seq.length s1 == rows * shared })
+  (s2 : (seq u64){ Seq.length s2 == shared * columns })
   (row: nat{row < rows}) (col: nat{col < columns}) (to: nat)
     : Lemma
       (requires (0 < to /\ to <= shared))
@@ -39,25 +39,25 @@ let matmul_single_lemma
 
 private let matmul_single_at
   (rows shared columns: nat)
-  (s1: (seq U64.t){ Seq.length s1 == rows * shared })
-  (s2 : (seq U64.t){ Seq.length s2 == shared * columns })
+  (s1: (seq u64){ Seq.length s1 == rows * shared })
+  (s2 : (seq u64){ Seq.length s2 == shared * columns })
   (idx: nat{idx < rows * columns})
-    : GTot U64.t
+    : GTot u64
   =
   let row = idx / columns in let col = idx % columns in matmul_single rows shared columns s1 s2 row col shared
 
 let matmul
   (rows shared columns: nat)
-  (s1: (seq U64.t){ Seq.length s1 == rows * shared })
-  (s2 : (seq U64.t){ Seq.length s2 == shared * columns })
-    : GTot (sr:(seq U64.t){ Seq.length sr == rows * columns })
+  (s1: (seq u64){ Seq.length s1 == rows * shared })
+  (s2 : (seq u64){ Seq.length s2 == shared * columns })
+    : GTot (sr:(seq u64){ Seq.length sr == rows * columns })
   =
   Seq.init_ghost (rows * columns) (matmul_single_at rows shared columns s1 s2)
 
 let lemma_matmul_index
   (rows shared columns: nat)
-  (s1: (seq U64.t){ Seq.length s1 == rows * shared })
-  (s2 : (seq U64.t){ Seq.length s2 == shared * columns })
+  (s1: (seq u64){ Seq.length s1 == rows * shared })
+  (s2 : (seq u64){ Seq.length s2 == shared * columns })
   (idx: nat{idx < rows * columns})
     : Lemma
       (ensures (Seq.index (reveal (matmul rows shared columns s1 s2)) idx) == reveal (matmul_single rows shared columns s1 s2 (idx / columns) (idx % columns) shared))
